Hints!
\begin{align}
&\dbd{\rho}{t}+\dbd{ }{x_j} \rho v_j = 0\\
&\dbd{v_i}{t} + v_j \dbd{ }{x_j} v_i = \frac{-1}{\rho}\dbd{ }{x_i} P\\
&\dbd{^2}{t}\rho -c_s^2 \dbd{^2 }{x^2} \rho = 0\\
&\dbd{v_i}{t} + v_j \dbd{ }{x_j} v_i = \frac{-1}{\rho}\dbd{ }{x_i} P + \nu \dbd{^2 }{x_j^2} v_i\\
&\omega^2 = g k \tanh(k d)\\
&\dbd{ }{t} v + v \dbd{ }{X} v + \sigma \dbd{^3}{X^3} v = 0\\
&\frac{\omega}{k} = \frac{ \rho U + \p{\rho}\p{U}}{\rho+\p{\rho}} \pm \sqrt{\frac{g}{k}\frac{\rho-\p{\rho}}{\rho+\p{\rho}}-\frac{ \rho\p{\rho}(U-\p{U})^2}{(\rho+\p{\rho})^2}} \end{align}
